theories/Syntax.v
@@ -56,8 +56,7 @@ Inductive gType  :=
   | GEnd : gType
   | GRec : gType -> gType
   | GMsg : action -> U -> gType-> gType
-  | GBranch : action  -> seq gType -> gType
-  | GPar : gType -> gType -> gType.
+  | GBranch : action  -> seq gType -> gType.
 Set Elimination Schemes. 
 
 Section Elimination.
@@ -70,7 +69,6 @@ Hypothesis Pg_end : Pg GEnd.
 Hypothesis Pg_rec : (forall g : gType, Pg g -> Pg (GRec g)).
 Hypothesis Pg_msg : (forall (a : action) (u : U) (g : gType), Pg g -> Pg (GMsg a u g)).
 Hypothesis Pg_branch : (forall (a : action) (l : seq gType), P_glist l  -> Pg (GBranch a l)).
-Hypothesis Pg_par : (forall g : gType, Pg g -> forall g0 : gType, Pg g0 -> Pg (GPar g g0)).
 
 Hypothesis P_glist_0 : P_glist nil.
 Hypothesis P_glist_cons : forall g, Pg g -> forall l, P_glist l -> P_glist (g::l).
@@ -88,7 +86,6 @@ fix gType_rect g :=
    | GRec g => Pg_rec (gType_rect g)
    | GMsg a u g => Pg_msg a u (gType_rect g)
    | GBranch a l => Pg_branch a (seq_gType_rect l)
-   | GPar g0 g1 => Pg_par (gType_rect g0) (gType_rect g1)
    end.
 
 Definition seq_gType_rect : forall gs, P_glist gs :=
@@ -110,109 +107,38 @@ Definition gType_choiceMixin := [derive choiceMixin for gType].
 Canonical gType_choiceType := ChoiceType gType gType_choiceMixin.
 Definition gType_countMixin := [derive countMixin for gType].
 Canonical gType_countType := CountType gType gType_countMixin.
-
 Check mut_rect.
-Definition gType_ind P := @mut_rect P (fun gs => forall g, List.In g gs -> P g).
-(*Lemma gType_ind :
-  forall (P : gType -> Prop),
-    P GEnd ->
-    (forall v, P (var_gType v)) ->
-    (forall G, P G -> P (GRec G)) ->
-    (forall a gs, (forall g, List.In g gs -> P g) -> P (GBranch a gs)) ->
-    (forall a u g0, P g0 -> P (GMsg a u g0)) ->
-    (forall g0 g1, P g0 -> P g1 -> P (GPar g0 g1)) ->
-    forall g : gType, P g.
-Proof.
-  move=> P P_end P_var P_rec P_branch P_msg P_par. fix Ih 1; case.
-  + by apply: P_var.
-  + by apply: P_end.
-  + by move=>G; apply: P_rec.
-  + move=> a s g; apply: P_msg. done. 
-  + move => a l. apply P_branch. intros. elim : l H. 
-   * simpl. contradiction. 
-   * move=> a0 l H. simpl. case. move =><-. apply Ih. done. 
-  + move => g g0. by apply : P_par. 
-Qed.*)
 
-(*
-Definition gType_der := [indDef for gType_ind].
+Definition gType_ind P := @gType_rect P (fun gs => forall (g : gType), true ).
 
-Fixpoint gType_eqb g0 g1 := 
-let list_eq := fix list_eq s1 s2 {struct s1} := 
-                                 match s1,s2 with
-                                  | [::] , [::] => true 
-                                  | x1 :: s1', x2 :: s2' =>  gType_eqb x1 x2 && (list_eq s1' s2') 
-                                  | _ , _ => false 
-                                  end
-in
-match g0, g1 with
-| GMsg a0 v0 g0', GMsg a0' v0' g1' => (a0 == a0') && (v0 == v0') && (gType_eqb g0' g1') 
-| GRec g0', GRec g1' => gType_eqb g0' g1' 
-| GEnd, GEnd => true
-| GPar g0' g0'', GPar g1' g1'' => (gType_eqb g0' g1') && (gType_eqb g0'' g1'')
-| GBranch a gs, GBranch a' gs' => (a == a') && (list_eq gs gs')
-| var_gType n, var_gType n' => n == n'
-| _, _ => false
-end.
-
-Ltac case_filter :=  case;try (rewrite /= ; constructor ; done);intros.
-Ltac case_filter_on x := generalize dependent x;case_filter.
-Ltac inj := split; solve [ by move/eqP=>-> | by case; move=>->].
-
-Ltac inject :=  split; [ by move=>-> | by case ].
-Ltac inject2 :=  split;[ case; by move =>->-> | case;by move =>->-> ]. 
-Ltac inject3 := split; [ case;  move=>->; case; move=>->->; done |  case; move =>->->->; done]. 
-
-
-
-Lemma reflexive_gType :  reflexive gType_eqb.
-Proof. unfold reflexive.
-elim;try solve [ rewrite /= ; done].
-- intros. rewrite /=. induction gs; first by rewrite eqxx.
-  rewrite eqxx /=. apply/andP. split. apply H. simpl. auto. 
-  have : (forall g, List.In g gs -> gType_eqb g g). intros. apply H. simpl; auto. 
-  move/IHgs. move/andP => [] _. done. 
-- intros. by rewrite /= !eqxx H. 
-- intros. by rewrite /= H H0.
+(*Remove vacously true sub goal from principle*)
+Lemma gType_ind_list P : 
+       (forall n : nat, P (GVar n)) ->
+       P GEnd ->
+       (forall g : gType, P g -> P (GRec g)) ->
+       (forall (a : action) (u : U) (g : gType), P g -> P (GMsg a u g)) ->
+       (forall (a : action) (l : seq gType),
+        (forall g : gType_eqType, g \in l -> P g) -> P (GBranch a l)) ->
+       (forall g : gType,
+        P g ->
+        forall l : seq gType,
+        (forall g0 : gType_eqType, g0 \in l -> P g0) ->
+        forall g0 : gType_eqType, g0 \in g :: l -> P g0) -> 
+       forall g : gType, P g.
+Proof. 
+intros. move : g. apply : (@gType_rect P (fun gs => forall g, g \in gs -> P g));auto.
+move => g. rewrite in_nil. done.
 Qed.
 
 
-Lemma gType_eqb_axiom : Equality.axiom gType_eqb.
-Proof.
-unfold Equality.axiom. intros.  apply Bool.iff_reflect.
-generalize dependent y. generalize dependent x.
-elim. 
-- case_filter.
-- move=>n. case_filter. rewrite /=. split. case; first by (move=>->; rewrite eqxx). 
-  move/eqP=>->. done.
-- move=> g Hg. case_filter. split. 
- * case; first (move=>->; rewrite /=). by rewrite reflexive_gType. 
- * rewrite /=. rewrite <- Hg. move=>->. done.
-- move => a gs H. case_filter. split.
- * case. move=>->->. by rewrite reflexive_gType. 
- * intros. f_equal. simpl in H0. by move : (andP H0) =>[]=>/eqP. simpl in H0. 
-   move : (andP H0)=>[] _. clear H0. generalize dependent l.  induction gs;case_filter.  done. 
-   done. 
-   move : (andP b). case. move/H=>H1 H2. rewrite H1. f_equal. apply IHgs. 
-   intros. apply H. simpl. auto. done. simpl;auto. 
--
- move=> a u g0 H. case_filter. split. case. move=>->->->. rewrite reflexive_gType. done.
- rewrite /=. move/andP=>[]/andP[]/eqP +/eqP=>->->. move/H=>->. done. 
-- move=> g0 g1 H0 H1. case_filter. rewrite /=. split. case. move=>->->.
-  rewrite !reflexive_gType. done.
-  move/andP=>[] /H0 + /H1=>->->.  done.
-Qed.
- 
-
-Definition gType_eqMixin := EqMixin gType_eqb_axiom. 
-Canonical gType_EqType := EqType gType gType_eqMixin.*)
+Definition gType_rec_list P := @gType_ind_list P. 
 
 Fixpoint bound_i (i : nat) (g : gType) := 
 match g with 
 | GEnd => true
 | GMsg _ _ g0 => bound_i i g0
 | GBranch _ gs => all (bound_i i) gs
-| GPar g0 g1 => (bound_i i g0) && (bound_i i g1)
+(*| GPar g0 g1 => (bound_i i g0) && (bound_i i g1)*)
 | GRec g0 => bound_i (S i) g0
 | GVar n => n < i
 end.
@@ -223,16 +149,12 @@ match g with
 | GEnd => true
 | GMsg _ _ g0 => contractive_i 0 g0
 | GBranch _ gs => all (contractive_i 0) gs
-| GPar g0 g1 => (contractive_i d g0) && (contractive_i d g1)
+(*| GPar g0 g1 => (contractive_i d g0) && (contractive_i d g1)*)
 | GRec g0 => contractive_i (S d) g0
 | GVar n => d <= n
 end. 
 
-(*
-Inductive wfgType n := WFgType g of bound_i n g && contractive_i 0 g.
-Coercion gType_of_wf n (wfg : wfgType n)  := let: WFgType g _ := wfg in g.
-Canonical wfgType_subType n := [subType for (@gType_of_wf n)].
-Definition GType := wfgType 0. *)
+
 
 Fixpoint substitution (i : nat) (g0 g1 : gType) :=
 match g0 with
@@ -240,7 +162,7 @@ match g0 with
 | GBranch a gs => GBranch a (map (fun g0' => substitution i g0' g1) gs)
 | GVar n => if n == i then g1 else g0
 | GRec g0' => GRec (substitution (S i) g0' g1)
-| GPar g0' g1' => GPar (substitution i g0' g1) (substitution i g1' g1)
+(*| GPar g0' g1' => GPar (substitution i g0' g1) (substitution i g1' g1) *)
 | GEnd => GEnd
 end.
 
@@ -253,7 +175,8 @@ Arguments substitution {_}.
 Notation bound := (bound_i 0).
 Notation contractive := (contractive_i 0).
 
-Notation "G '[' G0 ']'" := (substitution 0 G G0)(at level 0).
+Notation "G [ G0 ]" := (substitution 0 G G0)(at level 0, format "G [ G0 ]").
+
 Notation gt_pred := (fun n0 n1 g => bound_i n0 g && contractive_i n1 g).
 
 
@@ -263,9 +186,14 @@ Arguments GMsg {_}.
 Arguments GBranch {_}.
 Arguments GVar {_}.
 Arguments GRec {_}.
-Arguments GPar {_}.
+(*Arguments GPar {_}.*)
 Arguments GEnd {_}.
 
+Definition linear_spec := 
+forall (g0 g1 : gType U), (exists2 p, path (grel g_next) g p & g0 = last g p) ->
+                     (exists2 p, path (grel g_next) g p & g1 = last g p) ->
+                     (exists2 p, path (grel g_next) g0 p & g1 = last g0 p) ->
+                     opt_rel g0 g1 same_ch -> in_dep_spec g0 g1 /\ out_dep_spec g0 g1.
 
 
 
